\chapter{Results on Random Variables}
\begin{lemma}
	\label{lem:var_addition}
	If $X,Y$ are independent random variables, then
	\begin{equation*}
		\begin{split}
			\mathrm{Var}(X+Y) = \mathrm{Var}(X) + \mathrm{Var}(Y).
		\end{split}
	\end{equation*}
	\begin{proof}
		Without loss of generality, assume $X$ and $Y$ have mean $0$. Then
		\begin{equation*}
			\begin{split}
				\mathrm{Var}(X+Y) =  \mathrm{E}( (X + Y)^{2} ) & = \mathrm{E}(X^{2} + 2XY + Y^{2})
				\\
				& = \mathrm{E}(X^{2}) + 2 \mathrm{E}(X) \mathrm{E}(Y) + \mathrm{E}(Y^{2}) \quad \text{via independence}
				\\
				& = \mathrm{E}(X^{2}) + \mathrm{E}(Y^{2})
				\\
				& = \mathrm{Var}(X) + \mathrm{Var}(Y)
			\end{split}
		\end{equation*}

	\end{proof}

\end{lemma}
\begin{lemma}
	If $X_{1}, \cdots, X_{n}$ and $Y_{1}, \cdots, Y_{n}$ are independent samples
	generated by random variables $X, Y$,
	then
	\begin{equation*}
		\begin{split}
			\mathrm{SE}_{\bar{X} + \bar{Y}} = \mathrm{SE}_{\bar{X}}^{2} + \mathrm{SE}_{\bar{Y}}^{2}	
		\end{split}
	\end{equation*}

\end{lemma}
\begin{proof}
	\begin{equation*}
		\begin{split}
			\mathrm{SE}_{\bar{X} + \bar{Y}}^{2}
			& = \frac{1}{n}\sum_{i=1}^{n} \mathrm{Var}(x_{i} +
			y_{i}) \\
			& = \frac{1}{n}\sum_{i=1}^{n}\mathrm{Var}(x_{i}) +
			\frac{1}{n}\sum_{i=1}^{n}\mathrm{Var}(y_{i}) 
			\\
			& = \mathrm{SE}_{\bar{X}}^{2} + \mathrm{SE}_{\bar{Y}}^{2}
		\end{split}
	\end{equation*}
	where the second line follows from \Cref{lem:var_addition}.
\end{proof}

