%
%
\documentclass[12pt,reqno]{amsart}
\usepackage{amsmath}
\usepackage{amssymb}
\usepackage[notref, notcite]{showkeys}
\usepackage{cancel}  %for cancelling terms explicity on pdf
\usepackage{yhmath}   %makes fourier transform look nicer, among other things
\usepackage{framed}  %for framing remarks, theorems, etc.
\usepackage{enumerate} %to change enumerate symbols
\usepackage[margin=2.5cm]{geometry}  %page layout
\numberwithin{equation}{section}  %eliminate need for keeping track of counters
\setlength{\parindent}{0in} %no indentation of paragraphs after section title
\renewcommand{\baselinestretch}{1.1} %increases vert spacing of text
%
\usepackage{hyperref}
\hypersetup{colorlinks=true,
linkcolor=blue,
citecolor=blue,
urlcolor=blue,
}
\synctex=1
%\usepackage[alphabetic, initials, msc-links]{amsrefs} %for the bibliography;
%%uses cite pkg. Must be loaded after hyperref, otherwise doesn't work properly
%%(conflicts with cref in particular)
%
%
\newcommand{\ds}{\displaystyle}
\newcommand{\ts}{\textstyle}
\newcommand{\nin}{\noindent}
\newcommand{\rr}{\mathbb{R}}
\newcommand{\nn}{\mathbb{N}}
\newcommand{\zz}{\mathbb{Z}}
\newcommand{\cc}{\mathbb{C}}
\newcommand{\ci}{\mathbb{T}}
\newcommand{\zzdot}{\dot{\zz}}
\newcommand{\wh}{\widehat}
\newcommand{\p}{\partial}
\newcommand{\ee}{\varepsilon}
\newcommand{\vp}{\varphi}
\newcommand{\wt}{\widetilde}
%
%
%
%
\newtheorem{theorem}{Theorem}[section]
\newtheorem{lemma}[theorem]{Lemma}
\newtheorem{corollary}[theorem]{Corollary}
\newtheorem{claim}[theorem]{Claim}
\newtheorem{prop}[theorem]{Proposition}
\newtheorem{proposition}[theorem]{Proposition}
\newtheorem{no}[theorem]{Notation}
\newtheorem{definition}[theorem]{Definition}
\newtheorem{remark}[theorem]{Remark}
\newtheorem{examp}{Example}[section]
\newtheorem{exercise}[theorem]{Exercise}
%
%makes proof environment bold instead of italic
%\makeatletter
%\renewcommand\subsubsection{\@startsection{subsubsection}{3}{\z@}%
%{-3.25ex\@plus -1ex \@minus -.2ex}%
%{1.5ex \@plus .2ex}%
%{\normalfont\normalsize \bfseries}}
%\makeatother
%makes subsubsubsection bold instead of italic
%
\def\sgn{\operatorname{sgn}}
\newcommand{\uol}{u^\omega_\lambda}
\newcommand{\lbar}{\bar{l}}
\renewcommand{\l}{\lambda}
\newcommand{\R}{\mathbb{R}}
\newcommand{\RR}{\mathcal{R}}
\newcommand{\al}{\alpha}
\newcommand{\ve}{q}
\newcommand{\tg}{{tan}}
\newcommand{\m}{q}
\newcommand{\N}{N}
\newcommand{\ta}{{\tilde{a}}}
\newcommand{\tb}{{\tilde{b}}}
\newcommand{\tc}{{\tilde{c}}}
\newcommand{\tS}{{\tilde{S}}}
\newcommand{\tP}{{\tilde{P}}}
\newcommand{\tu}{{\tilde{u}}}
\newcommand{\tw}{{\tilde{w}}}
\newcommand{\tA}{{\tilde{A}}}
\newcommand{\tX}{{\tilde{X}}}
\newcommand{\tphi}{{\tilde{\phi}}}
\begin{document}
\title{Ill-Posedness for the Boussinesq Equation}
\author{Dan-Andrei Geba, Alexandrou Himonas, and David Karapetyan}
\address{Department of Mathematics, University of Rochester, Rochester, NY 14627}
\address{Department of Mathematics, University of Notre Dame, Notre Dame, IN 46556}
\address{Department of Mathematics, University of Notre Dame, Notre Dame, IN 46556}
\date{\today}
%
%
\maketitle
%
%
%
%
%%%%%%%%%%%%%%%%%%%%%%%%%%%%%%%%%%%%%%%%%%%%%%
%
%
%
%Ill-Posedness
%
%
%
%%%%%%%%%%%%%%%%%%%%%%%%%%%%
%
%
\section{Introduction}
Our motivation will be the work of Bejanaru and Tao
\cite{Bejenaru-Tao-2006-Sharp-well-posedness-and-ill-posedness}. 
%
\begin{definition}
  For $f =f(x)= (f_{1}(x), f_{2}(x)), u = u(x,t), v = v(x,t)$ formally define 
%
%
\begin{equation*}
\begin{split}
  L(f)
  \doteq \frac{1}{2 \pi} \psi(t) \sum_{n \in \zz} e^{inx}
  \wh{f_{1}}(n) \frac{e^{i\lambda(n)t} + e^{-i\lambda(n)t}}{2} 
  & + \psi(t) \sum_{n \in \zz} e^{inx}
  \wh{f_{2}}(n)\frac{e^{i\lambda(n)t} - e^{-i\lambda(n)t}}{2 i \lambda(n)} 
\end{split}
\end{equation*}
%
%
and
%
%
\begin{equation*}
\begin{split}
N(u, v)
& \doteq \frac{1}{4 \pi i} \psi_{\delta}(t) \sum_{n \in \zz} e^{inx} \frac{n^{2}}{\lambda(n)}
    \int_{0}^{t}[e^{i\lambda(n)(t-t')}-e^{-i\lambda(n)(t-t')}]
    \wh{uv}(n, t') dt'.
\end{split}
\end{equation*}
%
%
Then we let $A_{n}: H^{s} \times H^{s-2} \to C([-\delta, \delta], H^{s}), \ n = 1, 2, \dots$ be the
recursively defined maps
%
%
\begin{equation*}
\begin{split}
  & A_{1}(f) \doteq L(f),
  \\
  & A_{n}(f) \doteq \sum_{j, k \in \mathbb{N}: j + k = n} N\left[
  A_{j}(f), A_{k}(f) \right], \quad n > 1.
\end{split}
\end{equation*}
\end{definition}
%
%
%
For example, 
%
%
\begin{equation*}
\begin{split}
  & A_{2}(f_{N}) = N(A_{1}(f_{N}), A_{1}(f_{N}))
  \\
  & A_{3}(f_{N}) = N(A_{1}(f_{N}), A_{2}(f_{N})) + N(A_{2}(f_{N}), A_{2}(f_{N}))
  \\
  & A_{4}(f_{N})= N(A_{1}(f_{N}), A_{3}(f_{N})) + N(A_{2}(f_{N}), A_{2}(f_{N}))
  + N(A_{3}(f_{N}), A_{1}(f_{N}))
\end{split}
\end{equation*}
%
%
and so on. The key tool in our proof of ill-posedness is the assumption of
qualitative well-posedness for Boussinesq for $s \ge -1$, that is, well-posedness given by a picard iteration in a Banach space which is continuously embedded in $C([0, T], H^{s})$, where $T > 0$ depends on the $H^{s}$ size of the initial data. If qualitative well-posedness holds for $s \ge -1$, then for
initial data in $H^{s} \times H^{s-2}$, $s \ge -1$, the corresponding solution
to the Boussinesq ivp can be asymptotically expanded as the sum of the iterates defined
above. More precisely, we have the following.
%%
\begin{lemma}
  \label{lem:qwp-awp}
  Suppose the Boussinesq ivp is qualitatively well-posed for $s \ge -1$. Then for
  $f \in B_{H^{s} \times H^{s-2}}(r)$, $s \ge -1$,  and $\delta=\delta(r)$
sufficiently small, we have the absolutely convergent
(in $C([-\delta, \delta], H^{s})$) power series expansion
%
%
\begin{equation}
  \label{power-series-soln}
\begin{split}
  u[f] = \sum_{n=1}^{\infty} A_{n}(f).
\end{split}
\end{equation}
%
%
\label{lem:analytic-wp}
\end{lemma}
%
%
%
%
%%%%%%%%%%%%%%%%%%%%%%%%%%%%%%%%%%%%%%%%%%%%%%%%%%%%%
%
%
%				Proof of Ill-Posedness
%
%
%%%%%%%%%%%%%%%%%%%%%%%%%%%%%%%%%%%%%%%%%%%%%%%%%%%%%
%
%
\section{Ill-Posedness for $s < -1$ on the Circle (Failure of Continuity)} 
\label{sec:pf-ill-pos}
Given the machinery established in the introduction, we see that to prove failure of continuity of the Boussinesq data to solution map at $\vec{0} =
(0, 0)$, it will be enough to show the
following.
%
%
%
%
%
%%%%%%%%%%%%%%%%%%%%%%%%%%%%%%%%%%%%%%%%%%%%%%%%%%%%%
%
%
%                Failure of Continuity at 0
%
%
%%%%%%%%%%%%%%%%%%%%%%%%%%%%%%%%%%%%%%%%%%%%%%%%%%%%%
%
%
\begin{theorem}
  Let $N$ be a positive integer. Consider initial data $$f_{N}(x) =
  (f_{N,1}(x), f_{N,2}(x)) = \left ( \frac{r N}{2 \pi}\left[ e^{ix} + e^{i(N-1)x} \right], 0
  \right ).$$ Then 
  %
  %
    \begin{enumerate}[(I)]
      \item{$ f_{N} \in B_{H^{-1} \times H^{-3}}(r) \ \text{with associated
    solutions}
    \ u[f_{N}] = \sum_{n=1}^{\infty} A_{n}(f_{N}) \in C([-\delta, \delta],
    H^{-1})$}.
    \\
  \item
    $\|f_{N}\|_{H^{\beta} \times H^{\beta-2}} \to 0$ for $\beta < -1$ but 
    $ \displaystyle \frac{\|A_{2}[f_{N}]\|_{C( [-\delta, \delta], H^{\beta})}}{\| f_{N}
    \|_{H^{\beta}}}$ diverges.
\end{enumerate}
  %
  %
\label{thm:ill-pos}
\end{theorem}
%
%
%
%
%
%
%
%
%
%
%
\begin{proof}
  We first bound $A_{2}(f_{N})$ from below.
  Observe that $f_{N} \in C^{\infty}$. In particular
%
%
\begin{equation}
  \label{ill-pos-ce}
\begin{split}
  \wh{f_{N,1}}(n)
  & = r N\int_{\ci} [e^{-ix(n - N)} + e^{-ix(n - (N-1))}]  dx  
  \\ 
  & = 
  \begin{cases}
    2 \pi r N,  \quad  & n = N \ \text{or} \ n = N-1
    \\
     0, \quad  & \text{otherwise}.
  \end{cases}
\end{split}
\end{equation}
%
Hence
%
%
\begin{equation}
  \label{ill-pos-ced}
\begin{split}
  \| f_{N,1} \|_{H^{\beta}}
  & = \frac{2 \pi r N}{2 \pi} \left( \sum_{n \in \zz} (1 + | n |)^{2 \beta} |
  \wh{f_{N,1}}(n) |^{2} \right)^{1/2}
  \\
  & \sim rN^{\beta +1}.
\end{split}
\end{equation}
%
%
Therefore, from \eqref{ill-pos-ced} we see that 
\begin{equation*}
  \begin{split}
    & (f_{N,1}, 0) \in B_{H^{-1} \times H^{-3}}(r)
    \\
    & \|(f_{N,1}, 0)\|_{H^{\beta} \times H^{\beta -2}} \to 0 \ \text{for} \ \beta < -1.
    \end{split}
\end{equation*}
Note that since we have assumed well-posedness for the Boussinesq equation for $s
\ge -1$, and since $f_{N} \in B_{H^{-1} \times H^{-3}}(cr)$, the associated
solutions $u[f_{N}]$ have common lifespan $\delta$ \emph{which does not depend
on $N$}. Choose $r$ sufficiently small such that $\delta =1$.  
Observe that
%
%
\begin{equation*}
\begin{split}
  & \| A_{2}(f_{N}) \|_{C([-1, 1], H^{\beta})} 
  \\
& \ge \| A_{2}(f_{N}) \|_{C([0, 1], H^{\beta})} 
\\
  &  =  \| N[A_{1}(f_{N}), A_{1}(f_{N})] \|_{C([0, 1],
  H^{\beta})} 
  \\
  & = \sup_{0 \le t \le 1} \| \psi_{1}(t) (1 + | n |)^{\beta}
  \frac{1}{4 i \pi} \frac{n^{2}}{\lambda(n)}
  \int_{0}^{t} \left( e^{i\lambda(n)(t-t')} - e^{-i\lambda(n)(t-t')} \right)
  \wh{[L(f_{N})]^{2}}(n, t') dt' \|_{\ell^{2}_{n}}
  \\
  & \gtrsim \sup_{0 \le t \le 1} \| (1 + | n |)^{\beta}
  \int_{0}^{t} \sum_{n_{1}} \left( e^{i\lambda(n)(t-t')} - e^{-i\lambda(n)(t-t')} \right)
  \\
  & \times \wh{f_{N}}(n - n_{1})\left( e^{i\lambda(n - n_{1})t'} +
  e^{-i\lambda(n - n_{1})t'} \right)
  \wh{f_{N}}(n_{1})\left( e^{i \lambda(n_{1})t'} +
  e^{-i \lambda(n_{1})t'} \right) 
  dt' \|_{\ell^{2}_{n}}
  \\
  & \gtrsim | \sup_{0 \le t \le 1} 
  N^{\beta + 2} 
\int_{0}^{t} \left( e^{i\lambda(N)(t-t')} - e^{-i\lambda(N)(t-t')} \right)
  \\
  & \times \left( e^{i\lambda(N - 1)t'} +
  e^{-i\lambda(N - 1)t'} \right)
  \left( e^{i \lambda(1)t'} +
  e^{-i \lambda(1)t'} \right) 
  dt' | 
 \end{split}
\end{equation*}
%
%
where the last step follows from the inequality $\| a_{n} \|_{\ell^{2}} \ge | a_{N} |$, the symmetry of the convolution, and the definition of $f_{N}$. Distributing terms, and setting $t=1$, we bound below by 
%
%
\begin{equation}
  \label{pre-int-decay}
\begin{split}
  & N^{\beta+2} | \int_{0}^{1} e^{i \lambda(N)}
  \\
  & \times \left( e^{it'[\lambda(N-1) - \lambda(N) + \lambda(1)]}
 + e^{it'[\lambda(N-1) - \lambda(N) - \lambda(1)]} 
 + e^{it'[\lambda(1) - \lambda(N-1) + \lambda(N)]}
 + e^{it'[-\lambda(N-1) - \lambda(N) - \lambda(1)]}
  \right)
 \\ 
 & - e^{-i \lambda(N)}
  \\
  & \times \left( e^{it'[\lambda(N-1) + \lambda(N) + \lambda(1)]}
 + e^{it'[\lambda(N-1) + \lambda(N) - \lambda(1)]} 
 + e^{it'[\lambda(1) - \lambda(N-1) + \lambda(N)]}
 + e^{it'[-\lambda(N-1) + \lambda(N) - \lambda(1)]}
  \right) |
\end{split}
\end{equation}
%
Now
%
%
\begin{equation*}
\begin{split}
\lambda(N) - \lambda(N-1)
 & = \sqrt{N^{2} + N^{4}} - \sqrt{(N-1)^{2} + (N-1)^{4}} 
 \\
 & = O(N)
\end{split}
\end{equation*}
%
%
while
%
%
\begin{equation*}
\begin{split}
  \lambda(N) + \lambda(N-1) = O(N^{2}).
\end{split}
\end{equation*}
%
%
Hence, evaluating the integrand of \eqref{pre-int-decay} from $0$ to $1$, we obtain $O(N^{-1})$ and $O(N^{-2})$ terms. Discarding all $O(N^{-2})$ terms, we get
%
%
\begin{equation*}
\begin{split}
  & | e^{i \lambda(N)}\left( \frac{e^{i}[\lambda(N-1) - \lambda(N) + \lambda(1)] - 1}{i[\lambda(N-1) - \lambda(N) + \lambda(1)]} + 
  \frac{e^{i}[\lambda(N-1) - \lambda(N) - \lambda(1)] - 1}{i[\lambda(N-1) - \lambda(N) - \lambda(1)]} \right)
  \\
  & + e^{-i \lambda(N)}\left( \frac{e^{-i}[\lambda(N-1) - \lambda(N) - \lambda(1)] - 1}{i[\lambda(N-1) - \lambda(N) - \lambda(1)]} + 
  \frac{e^{-i}[\lambda(N-1) - \lambda(N) + \lambda(1)] - 1}{i[\lambda(N-1) - \lambda(N) + \lambda(1)]} \right)
  \\
  & \simeq \frac{\cos[\lambda(N-1) + \lambda(1)] - \cos \lambda(N)}{\lambda(N) - \lambda(N-1) - \lambda(1)} + \frac{\cos[\lambda(N-1) - \lambda(1)] - \cos \lambda(N)}{\lambda(N) - \lambda(N-1) + \lambda(1)} |. 
\end{split}
\end{equation*}
%
%
Let $N = N_{k}$ be a sequence increasing to $\infty$ such that $\cos \lambda(N_{k}) = 0$ for all $k \ge 0$. Then the above reduces to 
%
%
%
%
\begin{equation}
  \label{puy}
\begin{split}
  & | \frac{\cos[\lambda(N-1) + \sqrt{2}] }{\lambda(N) - \lambda(N-1) - \lambda(\sqrt{2})} + \frac{\cos[\lambda(N-1) - \lambda(\sqrt{2})] }{\lambda(N) - \lambda(N-1) + \lambda(\sqrt{2})} |
  \\
  & = | \frac{\left \{ \lambda(N) - \lambda(N-1) \right \}\left \{ \cos[\lambda(N-1) + \sqrt{2}] + \cos\left[ \lambda(N-1) - \sqrt{2} \right] \right \}}{[\lambda(N) - \lambda(N-1) - \sqrt{2}][\lambda(N) - \lambda(N-1) + \sqrt{2}]} |
  \\
  & = | \frac{2 \left \{ \lambda(N) - \lambda(N-1) \right \}\left \{ \cos\lambda(N-1) \cos \sqrt{2} - \sin\lambda(N-1) \sin \sqrt{2} \right \}}{[\lambda(N) - \lambda(N-1) - \sqrt{2}][\lambda(N) - \lambda(N-1) + \sqrt{2}]} |
  \\
  & = O(N^{-1})a_{n}
\end{split}
\end{equation}
%
%
where
%
%
\begin{equation*}
\begin{split}
  a_{n} \doteq | \cos\lambda(N-1) \cos \sqrt{2} - \sin\lambda(N-1) \sin \sqrt{2} |.
\end{split}
\end{equation*}
%
%
Notice that $a_{n}$ is divergent. Substituting \eqref{puy} into \eqref{pre-int-decay}, we see that 
%
%
\begin{equation*}
\begin{split}
\|A_{2}[f_{N}]\|_{C( [-\delta, \delta], H^{\beta})}
   \gtrsim O(N^{\beta+1}) a_{n}.
\end{split}
\end{equation*}
%
Therefore, recalling \eqref{ill-pos-ced}, we see that
%
%
\begin{equation*}
\begin{split}
\frac{\|A_{2}[f_{N}]\|_{C( [-\delta, \delta], H^{\beta})}}{\| f_{N}
\|_{H^{\beta}}} \ge c a_{n}, \qquad c > 0 
\end{split}
\end{equation*}
%
%
which diverges. This concludes the proof.
%
%
%
%
%
\end{proof}
%
%
\begin{framed}
\begin{remark}
 Since $\{a_{n}\}_{n}$ is divergent, and $a_{n} \ge 0$, it follows that for each $\ee > 0$ there exists an $N' = N'(\ee)$ such that for all $N > N'$, we have
  %
  %
  \begin{equation*}
  \begin{split}
    a_{N} > \ee/c
  \end{split}
  \end{equation*}
  %
  %
  and so
  %
  %
  \begin{equation*}
  \begin{split}
  \|A_{2}[f_{N}]\|_{C( [-\delta, \delta], H^{\beta})}
  > \ee {\| f_{N} \|_{H^{\beta}}}
  \end{split}
  \end{equation*}
  %
  %
  for all $N > N'$. Letting $N \to \infty$ then establishes the failure of continuity of the data to solution map at $0$.  
\label{rem:calc}
\end{remark}
\end{framed}
%
%
%
%
%
%%%%%%%%%%%%%%%%%%%%%%%%%%%%%%%%%%%%%%%%%%%%%%%%%%%%%%%%%
%
%
%
%Quadratic NLS
%
%
%%%%%%%%%%%%%%%%%%%%%%%%%%%%%%%%%
%
%
\section{Quadratic NLS: An Equation for which the BT method Works}
%
  We consider the quadratic non-linear Schr\"odinger equation (qNLS)
\begin{equation}\label{nls-quad}
\begin{split}
& i u_t + u_{xx} = u^2\\
& u(x, 0) = f \in H^s(\R) \\
\end{split}
\end{equation}
which has the localized integral formulation 
\begin{equation}\label{uln-2}
 u = L(f) + N(u,u)
 \end{equation}
where $L$ is the linear operator
\begin{equation}\label{Ldef}
  L(f)(t) := \eta(t) e^{it\partial_{xx}} f
\end{equation}
and $N$ is the bilinear operator
\begin{equation}\label{Ndef}
\begin{split}
N(u,v)(t) &:=
\eta(t) e^{it\partial_{xx}} \int_\R a(s) e^{-is\partial_{xx}}(u(s)v(s))\ ds\\
&+ \int_\R a(t-s) e^{i(t-s)\partial_{xx}}(u(s) v(s))\ ds
\end{split}
\end{equation}
%
where $\eta: \R \to \R$ is a smooth bump function such that $\eta(t) = 1$ for
$|t| \leq 1$ and $\eta(t) = 0$ for $|t| > 2$, and $a(t) := \frac{1}{2}
\sgn(t)\eta(t/5)$.  
%
Bejanaru and Tao proved the following well-posedness result.
\begin{theorem}[Local well-posedness in $H^{-1}(\R)$]\label{lwp}
 %
 %
 %
Let $r > 0$ be any radius, and let $B_r$ be the ball
$$ B_r := B_{H^{-1}(\R)}(0,r) := \{ u_0 \in H^{-1}(\R): \| u_0 \|_{H^{-1}(\R)} < r \}.$$
Then there exists a time $T > 0$ (in fact we obtain $T = \max(1, c r^{-1/2} )$ for some absolute constant $c>0$)
and a map $f \mapsto u[f]$ which is continuous from $B_r$ to $C([0,T],
H^{-1}(\rr))$, such that the
restriction of this map to $B_r \cap H^s(\R)$ (with the $H^s(\R)$ topology) maps continuously 
to $C([0,T], H^s(\rr))$ for any $s \geq -1$.  Furthermore, if $f$ lies in
a smooth space, say $B_r \cap H^3(\R)$, then $u[f]$ lies in $C([0, T], H^3) \cap
C^1([0,T], H^1(\rr))$ and
solves the equation \eqref{nls-quad} in the classical sense.   
\end{theorem}
%
%
Furthermore, as in the case of Boussinesq, solutions to the qNLS have an asymptotic
expansion in terms of iterates of the non-linearity. More precisely, they show
the following. 
%
\begin{lemma}
  \label{lem:qnls-asymp}
  For $f \in B_{H^{s}}(r)$, $s \ge -1$ and $\delta=\delta(r)$
sufficiently small, we have the absolutely convergent
(in $C([-\delta, \delta], H^{s})$) power series expansion
%
%
\begin{equation}
  \label{qnlspower-series-soln}
\begin{split}
  u[f] = \sum_{n=1}^{\infty} A_{n}(f)
\end{split}
\end{equation}
%
%
\end{lemma}
They then invoke this well-posedness result to prove ill-posedness for $s <
-1$ as follows.
%
%
%
%
\subsection{Proof of Ill-Posedness for $s < -1$} 
%
%
%
Fix $s < -1$; we may rescale the lifespan $\delta$ to equal $1$.  Suppose for contradiction
that the solution map $f \mapsto u[f]$ is continuous on $B_r$ (with the
$H^{-1}_x(\R)$ topology) to $C([0, 1], H^{-1}(\rr))$ 
(with the $C([0,1], H^{s}(\rr)$ topology). From 
Lemma~\ref{lem:qnls-asymp}, we conclude that the quadratic operator
$$ A_2: f \mapsto N_2(Lf, Lf)$$ 
restricted to $[0,1] \times \R$, is continuous from $B_r$ (with the $H^{-1}_x(\R)$ topology) 
to $C([0,1], H^{s}(\rr))$.  In particular, this implies that
$$ \sup_{0 \leq t\leq 1}\| A_2(f_N)(y) \|_{H^{s}(\R)} \to 0$$
whenever $f_N$ is a sequence of functions in $B_r$ which goes to zero in $H^{-1}_x(\R)$ norm.
The left-hand side can be expanded by \eqref{Ldef}, \eqref{Ndef} as
$$ \sup_{0 \leq t \leq 1} 
\| \int_0^t \exp(i(t-t')\partial_{xx})((\exp(it' \partial_{xx}) f_N)^2)\ dt' \|_{H^{s}(\R)}$$
which after taking Fourier transforms becomes
$$\sup_{0 \leq t \leq 1} 
\| \langle \xi \rangle^{s}
\int_0^t \int_\R \exp(-i(t-t')\xi^2) \exp(it' (\xi_1^2 + (\xi-\xi_1)^2) \hat f_N(\xi_1) \hat f_N(\xi-\xi_1)\ d\xi_1 dt'
\|_{L^2_\xi(\R)}.$$
Now let $N > 100$ be a large parameter, and set 
$$ \hat f_N := r N 1_{[-10,10]}(|\xi|-N) / 1000.$$
Then $f_N \in B_r$, and $\|f_N\|_{H^{-1}_x(\R)} \to 0$ as $N \to \infty$.  Thus,
from the well-posedness result Theorem~\ref{lwp} and the fact that
Lemma~\ref{lem:qnls-asymp}
holds for
the qNLS, we see that for continuity of the data to solution map to hold for $s < -1$ we must have
\begin{equation}\label{sin}
\sup_{0 \leq t \leq 1} \| \langle \xi \rangle^{s}
\int_0^t \int_\R \exp(-i(t-t')\xi^2) \exp(it' (\xi_1^2 + (\xi-\xi_1)^2) \hat f_N(\xi_1) \hat f_N(\xi-\xi_1)\ d\xi_1 dt'
\|_{L^2_\xi(\R)} \to 0
\end{equation}
as $N \to \infty$.
Now set $t := 1/100N^2$ and localize to the region where $-1 \leq \xi \leq 1$.  One can verify that
$$ \Re( \exp(-i(t-t')\xi^2) \exp(it' (\xi_1^2 + (\xi-\xi_1)^2) )) > 1/2$$
whenever $0 \leq t' \leq t$ and $\xi_1$ lives in the support of $f_{N}$, hence we obtain
$$ 
\| \langle \xi \rangle^{s}
\int_0^t \int_\R \exp(-i(t-t')\xi^2) \exp(it' (\xi_1^2 + (\xi-\xi_1)^2)) \hat f_N(\xi_1) \hat f_N(\xi-\xi_1)\ d\xi_1 dt'
\|_{L^2_\xi(\R)} \geq c r^2$$
for some $c > 0$.  But this contradicts \eqref{sin}. \qed
%
%
\bibliography{/Users/davidkarapetyan/math/bib-files/references.bib}
\bibliographystyle{amsalpha-custom}
\end{document}
