\section{Proofs of Lemmas and Estimates}
\begin{proof}[Proof of \eqref{schwartz-bound}] We first observe that
\begin{equation*}
  \begin{split}
    \wh{\psi_1}(0) = \int_\ci \psi_1 \ dt \le 2 \pi 
  \end{split}
\end{equation*}
%
%
while for $k \ge 0$, we use integration by parts to express the 
the Fourier transform of the periodic extension of $\psi_1$ 
in the following form
%
%
\begin{equation*}
  \begin{split}
    \wh{\psi_1}(\lambda) 
    & = \int_\ci e^{-i \lambda t} \psi_1 (t) \ dt
    = \frac{1}{\left( i \lambda \right)^k } \int_\ci e^{-i \lambda t} 
    \p_t^k \psi_1(t) \ dt
  \end{split}
\end{equation*}
%
%
which in conjunction with the estimate $\left( 1 + |\lambda|  \right)^{k } \le |2 \lambda|^k$ for $\lambda \in \mathbb{N}$ 
gives
%
%
\begin{equation*}
  \begin{split}
    \left( 1 + |\lambda| \right)^k |\wh{\psi_1}(\lambda)|
    & \le |2 \lambda|^k | \int_\ci e^{-i \lambda t} \psi_1(t) \ dt |
    \\
    & \le 2 ^k | \int_\ci e^{-i \lambda t} \p_t^k \psi_1(t) \ dt|
    \\
    & \le 2^k \int_\ci | \p_t^k \psi(t) | \ dt 
    \\
    & \le 2^k \cdot 2 \pi  \|\p_t^k \psi_1(t) \|_{L^\infty(\ci)}
    \\
    & = c_k  
  \end{split}
\end{equation*}
%
which completes the proof.
\end{proof}
%
%
%
\begin{proof}[Proof of \cref{cor:four-mult-est-dual}]
By duality,
%
%
\begin{equation}
  \label{1g}
  \begin{split}
    \|f\|_{L^{\frac{4}{3}}(\ci^2)}
    & = \sup_{g \in L^4(\ci^2)} 
    \frac{|\ \int_{\ci^2} f \bar{g} \ dx dt|}{\|g\|_{L^4(\ci^2)}}
    \\
    & \ge \frac{|\ \int_{\ci^2} f \bar{g} \ dx 
    dt|}{\|g\|_{L^4(\ci^2)}}, \qquad g \in L^4(\ci^2)
    \\
    &  =   \frac{|\sum_{m,n} \wh{f}(m,n) 
    \bar{\wh{g}}\left( m,n \right)| }{ 4 \pi^2 \|g\|_{L^4(\ci^2)}}
  \end{split}
\end{equation}
%
%
where the last step follows from Parseval's theorem. Choose $g$ such that
%
%
\begin{equation*}
  \begin{split}
    \wh{g}(m,n) = \left( 1 + |n - m^2| \right)^{-3/4} \wh{f}(m,n).
  \end{split}
\end{equation*}
%
%
Then by \cref{lem:four-mult-est},
%
%
\begin{equation*}
  \begin{split}
    \|g\|_{L^4(\ci^2)}
    & \le \|\left( 1 + |n-m^2| \right)^{-3/8} 
    \wh{g}(m,n) \|_{\ell^2(\zz^2)}
    \\
    & = \|\left( 1 + |n-m^2| \right)^{-3/8} 
    \left( 1 + |n - m^2| \right)^{-3/4} \wh{f}(m,n)  \|_{\ell^2(\zz^2)}
    \\
    & \lesssim \|f\|_{\ell^2(\ci^2)} < \infty.
  \end{split}
\end{equation*}
%
%
Therefore, substituting into \eqref{1g}, we obtain
%
%
\begin{equation*}
  \begin{split}
    \|f\|_{L^{4/3}(\ci^2)}
    & \ge \frac{\sum_{m,n} |\wh{f}(m,n)|^2 \left( 
    1 + |n-m^2| \right)^{-3/4}}{4 \pi^2 \|g\|_{L^4(\ci^2)}}
    \\
    & \ge \frac{\sum_{m,n} |\wh{f}(m,n)|^2 \left( 
    1 + |n-m^2| \right)^{-3/4}}{4 \pi^2 c \|\left( 1 + |n - m^2| 
    \right)^{3/8} \wh{g}(n,m) \|_{\ell^2(\zz^2)}}
    \\
    & = \frac{ \sum_{m,n} |\wh{f}(m,n)|^2 \left( 1 + |n - m| 
    \right)^{-3/4}}{4 \pi^2 c \left( \sum_{n,m} |\wh{f}(n,m)|^2 \left( 
    1 + |n-m^2| \right)^{-3/4} \right)^{1/2}}
    \\
    & \simeq \|\left( 1 + |n-m^2| \right)^{-3/8} \wh{f}(m,n) \|_{\ell^2(\zz^2)}
  \end{split}
\end{equation*}
%
%
completing the proof. 
\end{proof}
%
